Made changes to pattern matching, commiting now because I will try another way of implementing assumePublic/assertPublic

test/Example.v
@@ -41,6 +41,7 @@ From Katamaran Require Import
      Bitvector
      Semantics.Registers
      MicroSail.SymbolicExecutor
+     MicroSail.ShallowExecutor
      Symbolic.Solver
      Specification
      Program.
@@ -111,11 +112,11 @@ End Finite.
 Module Import ExampleBase <: Base.
   Import stdpp.finite.
 
-  #[export] Instance typedeclkit : TypeDeclKit :=
-    {| enumi := Enums;
-       unioni := Unions;
-       recordi := Records;
-    |}.
+  #[export] Instance typedeclkit : TypeDeclKit := ty.Build_TypeDeclKit.
+    (* {| enumi := Enums; *)
+    (*    unioni := Unions; *)
+    (*    recordi := Records; *)
+    (* |}. *)
 
   Definition enum_denote (E : Enums) : Set :=
     match E with
@@ -130,11 +131,11 @@ Module Import ExampleBase <: Base.
   Definition record_denote (R : Records) : Set :=
     match R with end.
 
-  #[export] Instance typedenotekit : TypeDenoteKit typedeclkit :=
-    {| enumt := enum_denote;
-       uniont := union_denote;
-       recordt := record_denote;
-    |}.
+  #[export] Instance typedenotekit : TypeDenoteKit typedeclkit := ty.Build_TypeDenoteKit _.
+  (*   {| enumt := enum_denote; *)
+  (*      uniont := union_denote; *)
+  (*      recordt := record_denote; *)
+  (*   |}. *)
 
   Definition union_constructors (U : Unions) : Set :=
     match U with
@@ -149,31 +150,31 @@ Module Import ExampleBase <: Base.
                          end
     end.
 
-  Definition union_unfold (U : unioni) : uniont U -> { K & Val (union_constructor_type U K) } :=
-    match U with
-    | either => fun Kv =>
-                  match Kv with
-                  | inl v => existT Left v
-                  | inr v => existT Right v
-                  end
-    end.
+  (* Definition union_unfold (U : unioni) : uniont U -> { K & Val (union_constructor_type U K) } := *)
+  (*   match U with *)
+  (*   | either => fun Kv => *)
+  (*                 match Kv with *)
+  (*                 | inl v => existT Left v *)
+  (*                 | inr v => existT Right v *)
+  (*                 end *)
+  (*   end. *)
 
-  Definition union_fold (U : unioni) : { K & Val (union_constructor_type U K) } -> uniont U :=
-    match U with
-    | either => fun Kv =>
-                  match Kv with
-                  | existT Left v  => inl v
-                  | existT Right v => inr v
-                  end
-    end.
+  (* Definition union_fold (U : unioni) : { K & Val (union_constructor_type U K) } -> uniont U := *)
+  (*   match U with *)
+  (*   | either => fun Kv => *)
+  (*                 match Kv with *)
+  (*                 | existT Left v  => inl v *)
+  (*                 | existT Right v => inr v *)
+  (*                 end *)
+  (*   end. *)
 
-  Definition record_field_type (R : recordi) : NCtx Empty_set Ty :=
-    match R with end.
+  (* Definition record_field_type (R : recordi) : NCtx Empty_set Ty := *)
+  (*   match R with end. *)
 
-  Definition record_fold (R : recordi) : NamedEnv Val (record_field_type R) -> recordt R :=
-    match R with end.
-  Definition record_unfold (R : recordi) : recordt R -> NamedEnv Val (record_field_type R) :=
-    match R with end.
+  (* Definition record_fold (R : recordi) : NamedEnv Val (record_field_type R) -> recordt R := *)
+  (*   match R with end. *)
+  (* Definition record_unfold (R : recordi) : recordt R -> NamedEnv Val (record_field_type R) := *)
+  (*   match R with end. *)
 
   #[export] Instance eqdec_enum_denote E : EqDec (enum_denote E) :=
     ltac:(destruct E; auto with typeclass_instances).
@@ -189,21 +190,23 @@ Module Import ExampleBase <: Base.
     ltac:(destruct R; auto with typeclass_instances).
 
   #[export,refine] Instance typedefkit : TypeDefKit typedenotekit :=
-    {| unionk         := union_constructors;
-       unionk_ty      := union_constructor_type;
-       unionv_fold    := union_fold;
-       unionv_unfold  := union_unfold;
-       recordf        := Empty_set;
-       recordf_ty     := record_field_type;
-       recordv_fold   := record_fold;
-       recordv_unfold := record_unfold;
-    |}.
-  Proof.
-    - abstract (now intros [] []).
-    - abstract (now intros [] [[]]).
-    - abstract (intros []).
-    - abstract (intros []).
+    ty.Build_TypeDefKit _ _.
   Defined.
+  (*   {| unionk         := union_constructors; *)
+  (*      unionk_ty      := union_constructor_type; *)
+  (*      unionv_fold    := union_fold; *)
+  (*      unionv_unfold  := union_unfold; *)
+  (*      recordf        := Empty_set; *)
+  (*      recordf_ty     := record_field_type; *)
+  (*      recordv_fold   := record_fold; *)
+  (*      recordv_unfold := record_unfold; *)
+  (*   |}. *)
+  (* Proof. *)
+  (*   - abstract (now intros [] []). *)
+  (*   - abstract (now intros [] [[]]). *)
+  (*   - abstract (intros []). *)
+  (*   - abstract (intros []). *)
+  (* Defined. *)
 
   #[export] Instance varkit : VarKit := DefaultVarKit.
 
@@ -221,16 +224,16 @@ Module Import ExampleProgram <: Program ExampleBase.
 
   Section FunDeclKit.
     Inductive Fun : PCtx -> Ty -> Set :=
-    | abs :        Fun [ "x" ∷ ty.int               ] ty.int
-    | cmp :        Fun [ "x" ∷ ty.int; "y" ∷ ty.int ] (ty.enum ordering)
-    | gcd :        Fun [ "x" ∷ ty.int; "y" ∷ ty.int ] ty.int
-    | gcdloop :    Fun [ "x" ∷ ty.int; "y" ∷ ty.int ] ty.int
-    | msum :       Fun [ "x" ∷ ty.union either; "y" ∷ ty.union either] (ty.union either)
-    | length {σ} : Fun [ "xs" ∷ ty.list σ           ] ty.int
+    (* | abs :        Fun [ "x" ∷ ty.int               ] ty.int *)
+    (* | cmp :        Fun [ "x" ∷ ty.int; "y" ∷ ty.int ] (ty.enum ordering) *)
+    (* | gcd :        Fun [ "x" ∷ ty.int; "y" ∷ ty.int ] ty.int *)
+    (* | gcdloop :    Fun [ "x" ∷ ty.int; "y" ∷ ty.int ] ty.int *)
+    (* | msum :       Fun [ "x" ∷ ty.union either; "y" ∷ ty.union either] (ty.union either) *)
+    (* | length {σ} : Fun [ "xs" ∷ ty.list σ           ] ty.int *)
     | fpthree16 :  Fun [ "sign" ∷ ty.bvec 1 ] (ty.bvec 16)
     | fpthree32 :  Fun [ "sign" ∷ ty.bvec 1 ] (ty.bvec 32)
     | fpthree64 :  Fun [ "sign" ∷ ty.bvec 1 ] (ty.bvec 64)
-    | bvtest    :  Fun [ "sign" ∷ ty.bvec 42 ] (ty.bvec 42)
+    | bvtest    :  Fun [ "x" :: ty.int ] ty.int
     .
 
     Definition 𝑭  : PCtx -> Ty -> Set := Fun.
@@ -246,22 +249,22 @@ Module Import ExampleProgram <: Program ExampleBase.
 
     Local Coercion stm_exp : Exp >-> Stm.
 
-    Local Notation "'`LT'" := (@exp_val _ (ty.enum ordering) LT).
-    Local Notation "'`GT'" := (@exp_val _ (ty.enum ordering) GT).
-    Local Notation "'`EQ'" := (@exp_val _ (ty.enum ordering) EQ).
-    Local Notation "'`Left' e" := (exp_union either Left e) (at level 10, e at level 9).
-    Local Notation "'`Right' e" := (exp_union either Right e) (at level 10, e at level 9).
+    (* Local Notation "'`LT'" := (@exp_val _ (ty.enum ordering) LT). *)
+    (* Local Notation "'`GT'" := (@exp_val _ (ty.enum ordering) GT). *)
+    (* Local Notation "'`EQ'" := (@exp_val _ (ty.enum ordering) EQ). *)
+    (* Local Notation "'`Left' e" := (exp_union either Left e) (at level 10, e at level 9). *)
+    (* Local Notation "'`Right' e" := (exp_union either Right e) (at level 10, e at level 9). *)
     Local Notation "'x'"   := (@exp_var _ "x" _ _) : exp_scope.
     Local Notation "'y'"   := (@exp_var _ "y" _ _) : exp_scope.
     Local Notation "'z'"   := (@exp_var _ "z" _ _) : exp_scope.
 
-    Definition fun_msum : Stm ["x" ∷ ty.union either; "y" ∷ ty.union either] (ty.union either) :=
-      stm_match_union_alt either x
-       (fun K =>
-          match K with
-          | Left  => MkAlt (pat_var "z") (`Left z)
-          | Right => MkAlt (pat_var "z") (y)%exp
-          end).
+    (* Definition fun_msum : Stm ["x" ∷ ty.union either; "y" ∷ ty.union either] (ty.union either) := *)
+    (*   stm_match_union_alt either x *)
+    (*    (fun K => *)
+    (*       match K with *)
+    (*       | Left  => MkAlt (pat_var "z") (`Left z) *)
+    (*       | Right => MkAlt (pat_var "z") (y)%exp *)
+    (*       end). *)
 
     Definition fun_fpthree' (e f : nat) : Stm [ "sign" ∷ ty.bvec 1 ] (ty.bvec (1 + e + f)) :=
       let: "exp" ∷ ty.bvec e := stm_val (ty.bvec e) bv.one in
@@ -292,46 +295,40 @@ Module Import ExampleProgram <: Program ExampleBase.
        let f := (n - (e + 1)) in
        fun_fpthree' e f)%nat.
 
-    Definition fun_bvtest : Stm [ "sign" ∷ ty.bvec 42 ] (ty.bvec 42) :=
-      let: "one" ∷ ty.bvec 42 := stm_val (ty.bvec 42) bv.one in
-      let: "zero" ∷ ty.bvec 42 := stm_val (ty.bvec 42) bv.zero in
-      exp_binop
-        bop.bvadd
-        (exp_binop bop.bvsub (exp_var "sign") (exp_var "one"))
-        (exp_binop
-           bop.bvadd
-           (exp_var "one")
-           (exp_var "zero"))
+    Definition fun_bvtest : Stm [ "x" :: ty.int ] ty.int :=
+      stm_exp (exp_var "x")
     .
+
+    Open Scope exp_scope.
 
     Definition FunDef {Δ τ} (f : Fun Δ τ) : Stm Δ τ :=
       Eval compute in
       match f in Fun Δ τ return Stm Δ τ with
-      | abs => if: exp_int 0 <= x then x else - x
-      | cmp => if: x < y then `LT else
-               if: x = y then `EQ else
-               if: x > y then `GT else
-               fail "cmp failed"
-      | gcd => "x" <- call abs x ;;
-               "y" <- call abs y ;;
-               call gcdloop x y
-      | gcdloop =>
-               let: "z" := call cmp x y in
-               match: z in ordering with
-               | LT => call gcdloop x (y - x)
-               | EQ => x
-               | GT => call gcdloop (x - y) y
-               end
-      | msum => fun_msum
-      | length => stm_match_list
-                    (exp_var "xs")
-                    (stm_val ty.int 0)
-                    "y" "ys" (let: "n" := call length (exp_var "ys") in exp_int 1 + exp_var "n")
+      (* | abs => stm_if (exp_int 0 <= x) x (- x) *)
+      (* | cmp => if: x < y then `LT else *)
+      (*          if: x = y then `EQ else *)
+      (*          if: x > y then `GT else *)
+      (*          fail "cmp failed" *)
+      (* | gcd => "x" <- call abs x ;; *)
+      (*          "y" <- call abs y ;; *)
+      (*          call gcdloop x y *)
+      (* | gcdloop => *)
+      (*          let: "z" := call cmp x y in *)
+      (*          match: z in ordering with *)
+      (*          | LT => call gcdloop x (y - x) *)
+      (*          | EQ => x *)
+      (*          | GT => call gcdloop (x - y) y *)
+      (*          end *)
+      (* | msum => fun_msum *)
+      (* | length => stm_match_list *)
+      (*               (exp_var "xs") *)
+      (*               (stm_val ty.int 0) *)
+      (*               "y" "ys" (let: "n" := call length (exp_var "ys") in exp_int 1 + exp_var "n") *)
       | fpthree16 => fun_fpthree16
       | fpthree32 => fun_fpthree32
       | fpthree64 => fun_fpthree64
       | bvtest => fun_bvtest
-      end.
+      end%exp.
   End FunDefKit.
 
   Include DefaultRegStoreKit ExampleBase.
@@ -365,84 +362,85 @@ Module Import ExampleSpecification <: Specification ExampleBase ExampleSig Examp
     Import asn.notations.
     Notation asn_prop Σ P := (asn.formula (@formula_prop Σ Σ (sub_id Σ) P)).
 
-    Definition sep_contract_abs : SepContract [ "x" ∷ ty.int ] ty.int :=
-      {| sep_contract_logic_variables := ["x" ∷ ty.int];
-         sep_contract_localstore      := [term_var "x"];
-         sep_contract_precondition    := ⊤;
-         sep_contract_result          := "result";
-         sep_contract_postcondition   :=
-           asn_prop
-             ["x" ∷ ty.int; "result" ∷ ty.int]
-             (fun x result => result = Z.abs x)%type
-      |}.
+    (* Definition sep_contract_abs : SepContract [ "x" ∷ ty.int ] ty.int := *)
+    (*   {| sep_contract_logic_variables := ["x" ∷ ty.int]; *)
+    (*      sep_contract_localstore      := [term_var "x"]; *)
+    (*      sep_contract_precondition    := ⊤; *)
+    (*      sep_contract_result          := "result"; *)
+    (*      sep_contract_postcondition   := *)
+    (*        asn_prop *)
+    (*          ["x" ∷ ty.int; "result" ∷ ty.int] *)
+    (*          (fun x result => result = Z.abs x)%type *)
+    (*   |}. *)
 
-    Definition sep_contract_cmp : SepContract ["x" ∷ ty.int; "y" ∷ ty.int] (ty.enum ordering)  :=
-       {| sep_contract_logic_variables := ["x" ∷ ty.int; "y" ∷ ty.int];
-          sep_contract_localstore      := [term_var "x"; term_var "y"];
-          sep_contract_precondition    := ⊤;
-          sep_contract_result          := "result";
-          sep_contract_postcondition   :=
-            asn.match_enum
-              ordering (term_var "result")
-              (fun result =>
-                 match result with
-                 | LT => term_var "x" < term_var "y"
-                 | EQ => term_var "x" = term_var "y"
-                 | GT => term_var "x" > term_var "y"
-                 end)
-       |}.
+    (* Definition sep_contract_cmp : SepContract ["x" ∷ ty.int; "y" ∷ ty.int] (ty.enum ordering)  := *)
+    (*    {| sep_contract_logic_variables := ["x" ∷ ty.int; "y" ∷ ty.int]; *)
+    (*       sep_contract_localstore      := [term_var "x"; term_var "y"]; *)
+    (*       sep_contract_precondition    := ⊤; *)
+    (*       sep_contract_result          := "result"; *)
+    (*       sep_contract_postcondition   := *)
+    (*         asn.match_enum *)
+    (*           ordering (term_var "result") *)
+    (*           (fun result => *)
+    (*              match result with *)
+    (*              | LT => term_var "x" < term_var "y" *)
+    (*              | EQ => term_var "x" = term_var "y" *)
+    (*              | GT => term_var "x" > term_var "y" *)
+    (*              end) *)
+    (*    |}. *)
 
-    Definition sep_contract_gcd : SepContract [ "x" ∷ ty.int; "y" ∷ ty.int ] ty.int :=
-      {| sep_contract_logic_variables := ["x" ∷ ty.int; "y" ∷ ty.int];
-         sep_contract_localstore      := [term_var "x"; term_var "y"];
-         sep_contract_precondition    := ⊤;
-         sep_contract_result          := "result";
-         sep_contract_postcondition   :=
-           asn_prop
-             ["x" ∷ ty.int; "y" ∷ ty.int; "result" ∷ ty.int]
-             (fun x y result => result = Z.gcd x y)%type
-      |}.
+    (* Definition sep_contract_gcd : SepContract [ "x" ∷ ty.int; "y" ∷ ty.int ] ty.int := *)
+    (*   {| sep_contract_logic_variables := ["x" ∷ ty.int; "y" ∷ ty.int]; *)
+    (*      sep_contract_localstore      := [term_var "x"; term_var "y"]; *)
+    (*      sep_contract_precondition    := ⊤; *)
+    (*      sep_contract_result          := "result"; *)
+    (*      sep_contract_postcondition   := *)
+    (*        asn_prop *)
+    (*          ["x" ∷ ty.int; "y" ∷ ty.int; "result" ∷ ty.int] *)
+    (*          (fun x y result => result = Z.gcd x y)%type *)
+    (*   |}. *)
 
-    Definition sep_contract_gcdloop : SepContract [ "x" ∷ ty.int; "y" ∷ ty.int ] ty.int :=
-      {| sep_contract_logic_variables := ["x" ∷ ty.int; "y" ∷ ty.int];
-         sep_contract_localstore      := [term_var "x"; term_var "y"];
-         sep_contract_precondition    :=
-           term_val ty.int 0 <= term_var "x" ∗
-           term_val ty.int 0 <= term_var "y";
-         sep_contract_result          := "result";
-         sep_contract_postcondition   :=
-           asn_prop
-             ["x" ∷ ty.int; "y" ∷ ty.int; "result" ∷ ty.int]
-             (fun x y result => result = Z.gcd x y)%type
-      |}.
+    (* Definition sep_contract_gcdloop : SepContract [ "x" ∷ ty.int; "y" ∷ ty.int ] ty.int := *)
+    (*   {| sep_contract_logic_variables := ["x" ∷ ty.int; "y" ∷ ty.int]; *)
+    (*      sep_contract_localstore      := [term_var "x"; term_var "y"]; *)
+    (*      sep_contract_precondition    := *)
+    (*        term_val ty.int 0 <= term_var "x" ∗ *)
+    (*        term_val ty.int 0 <= term_var "y"; *)
+    (*      sep_contract_result          := "result"; *)
+    (*      sep_contract_postcondition   := *)
+    (*        asn_prop *)
+    (*          ["x" ∷ ty.int; "y" ∷ ty.int; "result" ∷ ty.int] *)
+    (*          (fun x y result => result = Z.gcd x y)%type *)
+    (*   |}. *)
 
-    Definition length_post {σ} (xs : list (Val σ)) (result : Val ty.int) :=
-      (result = Z.of_nat (@Datatypes.length (Val σ) xs))%type.
-    Definition sep_contract_length {σ} : SepContract [ "xs" ∷ ty.list σ ] ty.int :=
-      {| sep_contract_logic_variables := ["xs" ∷ ty.list σ ];
-         sep_contract_localstore      := [term_var "xs"];
-         sep_contract_precondition    := ⊤;
-         sep_contract_result          := "result";
-         sep_contract_postcondition   := asn_prop ["xs"∷ty.list σ; "result"∷ty.int] length_post
-      |}.
+    (* Definition length_post {σ} (xs : list (Val σ)) (result : Val ty.int) := *)
+    (*   (result = Z.of_nat (@Datatypes.length (Val σ) xs))%type. *)
+    (* Definition sep_contract_length {σ} : SepContract [ "xs" ∷ ty.list σ ] ty.int := *)
+    (*   {| sep_contract_logic_variables := ["xs" ∷ ty.list σ ]; *)
+    (*      sep_contract_localstore      := [term_var "xs"]; *)
+    (*      sep_contract_precondition    := ⊤; *)
+    (*      sep_contract_result          := "result"; *)
+    (*      sep_contract_postcondition   := asn_prop ["xs"∷ty.list σ; "result"∷ty.int] length_post *)
+    (*   |}. *)
 
-    Definition sep_contract_bvtest : SepContract [ "sign" ∷ ty.bvec 42 ] (ty.bvec 42) :=
-      {| sep_contract_logic_variables := ["sign" ∷ ty.bvec 42 ];
-         sep_contract_localstore      := [term_var "sign"];
-         sep_contract_precondition    := ⊤;
-         sep_contract_result          := "result";
-         sep_contract_postcondition   := asn.formula (formula_relop bop.eq (term_var "result") (term_var "sign"))
+    Definition sep_contract_bvtest : SepContract [ "x" ∷ ty.int ] ty.int :=
+      {|
+        sep_contract_logic_variables := ["x" ∷ ty.int];
+        sep_contract_localstore      := [term_var "x"];
+        sep_contract_precondition    := asn.formula (formula_public (term_var "x"));
+        sep_contract_result          := "result";
+        sep_contract_postcondition   := asn.formula (formula_public (term_var "result"))
       |}.
 
     Definition CEnv : SepContractEnv :=
       fun Δ τ f =>
         match f with
-        | abs       => Some sep_contract_abs
-        | cmp       => Some sep_contract_cmp
-        | gcd       => Some sep_contract_gcd
-        | gcdloop   => Some sep_contract_gcdloop
-        | msum      => None
-        | length    => Some sep_contract_length
+        (* | abs       => Some sep_contract_abs *)
+        (* | cmp       => Some sep_contract_cmp *)
+        (* | gcd       => Some sep_contract_gcd *)
+        (* | gcdloop   => Some sep_contract_gcdloop *)
+        (* | msum      => None *)
+        (* | length    => Some sep_contract_length *)
         | fpthree16 => None
         | fpthree32 => None
         | fpthree64 => None
@@ -463,6 +461,8 @@ End ExampleSpecification.
 
 Module Import ExampleExecutor :=
   MakeExecutor ExampleBase ExampleSig ExampleProgram ExampleSpecification.
+
+Compute SStoreSpec.exec_aux _ _ _ (FunDef bvtest).
 
 Local Ltac solve :=
   repeat
@@ -493,15 +493,25 @@ Local Ltac solve :=
     ).
 
 Goal True. idtac "Timing before: example/length". Abort.
-Lemma valid_contract_length {σ} : Symbolic.ValidContract (@sep_contract_length σ) (FunDef length).
-Proof. constructor. compute - [length_post Val Z.add]. solve; lia. Qed.
-Goal True. idtac "Timing after: example/length". Abort.
+(* Lemma valid_contract_length {σ} : Symbolic.ValidContract (@sep_contract_length σ) (FunDef length). *)
+(* Proof. constructor. compute - [length_post Val Z.add]. solve; lia. Qed. *)
+(* Goal True. idtac "Timing after: example/length". Abort. *)
 
-Goal True. idtac "Timing before: example/cmp". Abort.
-Lemma valid_contract_cmp : Symbolic.ValidContractReflect sep_contract_cmp (FunDef cmp).
-Proof. reflexivity. Qed.
-Goal True. idtac "Timing after: example/cmp". Abort.
-Lemma valid_contract_bvtest : Symbolic.ValidContractWithErasure sep_contract_bvtest (FunDef bvtest).
+(* Goal True. idtac "Timing before: example/cmp". Abort. *)
+(* Lemma valid_contract_cmp : Symbolic.ValidContractReflect sep_contract_cmp (FunDef cmp). *)
+(* Proof. reflexivity. Qed. *)
+(* Goal True. idtac "Timing after: example/cmp". Abort. *)
+(* Lemma valid_contract_bvtest : Symbolic.ValidContractWithErasure sep_contract_bvtest (FunDef bvtest). *)
+(* Proof. *)
+(*   now cbv. *)
+(* Qed. *)
+
+Module Import ExampleShallowExecutor :=
+  MakeShallowExecutor ExampleBase ExampleSig ExampleProgram ExampleSpecification.
+
+Compute vcgen 0 sep_contract_bvtest (FunDef bvtest).
+
+Lemma zerotest : vcgen 0 sep_contract_bvtest (FunDef bvtest).
 Proof.
   now cbv.
 Qed.
