theories/Syntax/Formulas.v
@@ -66,11 +66,14 @@ Module Type FormulasOn
   | formula_true
   | formula_false
   | formula_and (F1 F2 : Formula Σ)
-  | formula_or (F1 F2 : Formula Σ).
+  | formula_or (F1 F2 : Formula Σ)
+  | formula_public {σ} (t : Term Σ σ)
+  .
   #[global] Arguments formula_user {_} p ts.
   #[global] Arguments formula_bool {_} t.
   #[global] Arguments formula_true {_}.
   #[global] Arguments formula_false {_}.
+  #[global] Arguments formula_public {_ _} t.
 
 
   (* TODO: I don't know what we use this one for, so I don't know whether I need a change it so the whole conjuction is negated or each of the two sides is negated, but still a conjunction. *)
@@ -98,6 +101,7 @@ Module Type FormulasOn
       | formula_false          => formula_false
       | formula_and F1 F2      => formula_and (sub_formula F1 ζ) (sub_formula F2 ζ)
       | formula_or F1 F2       => formula_or (sub_formula F1 ζ) (sub_formula F2 ζ)
+      | formula_public t       => formula_public (subst t ζ)
       end.
 
   #[export] Instance substlaws_formula : SubstLaws Formula.
@@ -111,27 +115,35 @@ Module Type FormulasOn
       }
   Qed.
 
-  #[export] Instance instprop_formula : InstProp Formula.
-  Proof.
-  Admitted.
-    (* fix inst_formula {Σ} (fml : Formula Σ) (ι : Valuation Σ) := *)
-    (*   match fml with *)
-    (*   | formula_user p ts      => env.uncurry (𝑷_inst p) (inst ts ι) *)
-    (*   | formula_bool t         => inst (A := RelVal ty.bool) t ι = ty.SyncVal ty.bool true *)
-    (*   | formula_prop ζ P       => uncurry_named P (inst ζ ι) *)
-    (*   | formula_relop op t1 t2 => bop.eval_relop_propRel op (inst t1 ι) (inst t2 ι) *)
-    (*   | formula_true           => True *)
-    (*   | formula_false          => False *)
-    (*   | formula_and F1 F2      => inst_formula F1 ι /\ inst_formula F2 ι *)
-    (*   | formula_or F1 F2       => inst_formula F1 ι \/ inst_formula F2 ι *)
-    (*   end. *)
+  Definition isSync {σ} (rv : ty.RelVal σ) : Prop :=
+    match rv with
+    | ty.SyncVal _ _ => True
+    | ty.NonSyncVal _ _ _ => False
+    end.
+
+  #[export] Instance instprop_formula : InstProp Formula :=
+    fix inst_formula {Σ} (fml : Formula Σ) (ι : Valuation Σ) :=
+      match fml with
+      | formula_user p ts      => env.uncurry (𝑷_inst p) (inst ts ι)
+      | formula_bool t         => inst (A := RelVal ty.bool) t ι = ty.SyncVal ty.bool true
+      | formula_prop ζ P       => uncurry_named P (inst ζ ι)
+      | formula_relop op t1 t2 => match bop.eval_relop_propRel op (inst t1 ι) (inst t2 ι) with
+                                  | Some p => p
+                                  | None => False
+                                  end
+      | formula_true           => True
+      | formula_false          => False
+      | formula_and F1 F2      => inst_formula F1 ι /\ inst_formula F2 ι
+      | formula_or F1 F2       => inst_formula F1 ι \/ inst_formula F2 ι
+      | formula_public t       => isSync (inst t ι)
+      end.
 
   #[export] Instance instprop_subst_formula : InstPropSubst Formula.
   Proof.
     intros ? ? ? ? f. induction f; cbn; rewrite ?inst_subst; auto.
-  (*   now apply and_iff_morphism. now apply or_iff_morphism. *)
-  (* Qed. *)
-    Admitted.
+    now apply and_iff_morphism. now apply or_iff_morphism.
+  Qed.
+
 
   (* TODO: This is currently not true, either we leave it out if we don't need it, we change the definition of formula_relop_neg (see comment there) or the content of this lemma *)
   (* Lemma instprop_formula_relop_neg {Σ σ} (ι : Valuation Σ) (op : RelOp σ) : *)
@@ -151,21 +163,15 @@ Module Type FormulasOn
 
     #[export] Instance proper_formula_user [Σ p] :
       Proper (base.equiv ==> (⊣⊢)) (@formula_user Σ p).
-    Proof. intros xs ys xys ι; cbn.
-           (* now rewrite xys. Qed. *)
-           Admitted.
+    Proof. intros xs ys xys ι; cbn; now rewrite xys. Qed.
 
     #[export] Instance proper_formula_bool [Σ] :
       Proper (base.equiv ==> (⊣⊢)) (@formula_bool Σ).
-    Proof. intros s t e ι; cbn.
-           (* now rewrite e. Qed. *)
-           Admitted.
+    Proof. intros s t e ι; cbn; now rewrite e. Qed.
 
     #[export] Instance proper_formula_relop [Σ σ] (rop : RelOp σ) :
       Proper (base.equiv ==> base.equiv ==> (⊣⊢)) (@formula_relop Σ σ rop).
-    Proof. intros s1 t1 e1 s2 t2 e2 ι; cbn.
-           (* now rewrite e1, e2. Qed. *)
-    Admitted.
+    Proof. intros s1 t1 e1 s2 t2 e2 ι; cbn; now rewrite e1, e2. Qed.
 
     Lemma syncValEqIffEq {σ a b} : ty.SyncVal σ a = ty.SyncVal σ b <-> a = b.
     Proof.
@@ -179,12 +185,11 @@ Module Type FormulasOn
     Proof.
       intro ι. cbn. destruct (inst t1 ι); destruct (inst t2 ι).
       all: repeat rewrite syncValEqIffEq; cbn.
-    (*   - rewrite andb_true_iff; intuition. *)
-    (*   - split; intros. congruence. destruct H. congruence. *)
-    (*   - split; intros. congruence. destruct H. congruence. *)
-    (*   - split; intros. congruence. destruct H. congruence.   *)
-    (* Qed. *)
-      Admitted.
+      - rewrite andb_true_iff; intuition.
+      - split; intros. congruence. destruct H. congruence.
+      - split; intros. congruence. destruct H. congruence.
+      - split; intros. congruence. destruct H. congruence.  
+    Qed.
     #[local] Hint Rewrite formula_bool_and : katamaran.
 
 
@@ -211,33 +216,23 @@ Module Type FormulasOn
       formula_relop (Σ:=Σ) op (term_val σ v1) (term_val σ v2) ⊣⊢
       if bop.eval_relop_val op v1 v2 then formula_true else formula_false.
     Proof.
-      intro. cbn.
-      (* rewrite bop.eval_relop_equiv. *)
-    (*   now destruct bop.eval_relop_val. *)
-    (* Qed. *)
-      Admitted.
+      intro. cbn. rewrite bop.eval_relop_equiv.
+      now destruct bop.eval_relop_val.
+    Qed.
 
     Lemma formula_and_l [Σ] (F1 F2 : Formula Σ) : formula_and F1 F2 ⊢ F1.
-    Proof. intros ι H.
-           (* apply H. Qed. *)
-           Admitted.
+    Proof. intros ι H. apply H. Qed.
 
     Lemma formula_and_r [Σ] (F1 F2 : Formula Σ) : formula_and F1 F2 ⊢ F2.
-    Proof. intros ι H.
-           (* apply H. Qed. *)
-           Admitted.
+    Proof. intros ι H. apply H. Qed.
 
     Lemma unsatisfiable_formula_bool [Σ] (t : Term Σ ty.bool) :
       base.equiv t (term_val ty.bool false) -> Unsatisfiable (formula_bool t).
-    Proof. intros e ι. specialize (e ι). cbn in *.
-           (* congruence. Qed. *)
-           Admitted.
+    Proof. intros e ι. specialize (e ι). cbn in *. congruence. Qed.
 
     Lemma unsatisfiable_formula_false [Σ] :
       Unsatisfiable (@formula_false Σ).
-    Proof. unfold Unsatisfiable; intuition.
-    (* Qed. *)
-           Admitted.
+    Proof. unfold Unsatisfiable; intuition. Qed.
 
   End Reasoning.
 
@@ -259,6 +254,7 @@ Module Type FormulasOn
       | formula_or F1 F2       => F1' <- oc xIn F1 ;;
                                   F2' <- oc xIn F2 ;;
                                   Some (formula_or F1' F2')
+      | formula_public t       => option.map formula_public (occurs_check xIn t)
       end.
 
   #[export] Instance occurs_check_laws_formula : OccursCheckLaws Formula.
@@ -271,15 +267,11 @@ Module Type FormulasOn
 
     Lemma formula_cons_true [Σ] (k : PathCondition Σ) :
       k ▻ formula_true ⊣⊢ k.
-    Proof. symmetry.
-           (* now apply snoc_cancel. Qed. *)
-           Admitted.
+    Proof. symmetry. now apply snoc_cancel. Qed.
 
     Lemma formula_snoc_and [Σ] (k : PathCondition Σ) (F1 F2 : Formula Σ) :
       k ▻ formula_and F1 F2 ⊣⊢ k ▻ F1 ▻ F2.
-    Proof. intro ι. cbn. intuition.
-    (* Qed. *)
-           Admitted.
+    Proof. intro ι. cbn. intuition. Qed.
 
     Equations(noeqns) formula_eqs_ctx {Δ : Ctx Ty} {Σ : LCtx}
       (δ δ' : Env (Term Σ) Δ) : PathCondition Σ :=
